# Notes from 2024-05-24
## Fibonacci example with tail recursion
- Always remember that tail recursion converts you recursive function to an iterative solution at compiler level, so design your tail recursion function in a way that imitates iterative solution.
- This is how you do fibonacci iteratively.
```kotlin
fun fibIteratively(num:Int): Int {
    var curr = 1
    var prev = 0
    for(i in 1..num){
        val temp = prev
        prev = prev + curr
        curr = temp
    }
    return prev
}

@Test
fun testFibIteratively() {
    assertEquals(1, fibIteratively(1))
    assertEquals(1, fibIteratively(2))
    assertEquals(2, fibIteratively(3))
    assertEquals(3, fibIteratively(4))
    assertEquals(5, fibIteratively(5))
}
```
- Let's convert this to tail recursion.
```kotlin
fun fibTailRec(num:Int): Int{
    tailrec fun fibonacci(i:Int, curr:Int, prev:Int): Int{
        if(i == 0)
        {
            return prev
        }
        return fibonacci(i = i - 1, curr = prev, prev= prev+curr)
    }
    return fibonacci(i = num, curr = 1, prev = 0)
}

@Test
fun testFibTailRec() {
    assertEquals(1, fibTailRec(1))
    assertEquals(1, fibTailRec(2))
    assertEquals(2, fibTailRec(3))
    assertEquals(3, fibTailRec(4))
    assertEquals(5, fibTailRec(5))
}
```
- You can see the iterative approach could be copied 1:1 in a tail recursive way.